{
	"@id": "iot:PhaseToNeutralVoltageA",
	"@type": "rdfs:Class",
	"rdfs:comment": "The voltage between the phase (line) A and neutral (there exist phases A, B, and C).",
	"rdfs:label": "PhaseToNeutralVoltageA",
	"rdfs:subClassOf": { "@id": "iot:Property" },
	"iot:providesOutputData": {
		"@id": "iot:VoltageData"
	},
	"iot:writable" : "schema:False",
	"iot:observable" : "schema:Boolean"
},
{
	"@id": "iot:VoltageData",
	"@type": "rdfs:Class",
	"rdfs:comment": "Voltage data.",
	"rdfs:label": "VoltageData",
	"rdfs:subClassOf": { "@id": "schema:PropertyValue" },
	"schema:propertyType": { "@id": "schema:Float" },
	"schema:unitCode": { "@id": "iot:VoltageUnit" },
	"schema:minValue": "schema:Float",
	"schema:maxValue": "schema:Float"
},
{
	"@id": "iot:PhaseToNeutralVoltageB",
	"@type": "rdfs:Class",
	"rdfs:comment": "The voltage between the phase (line) B and neutral (there exist phases A, B, and C).",
	"rdfs:label": "PhaseToNeutralVoltageB",
	"rdfs:subClassOf": { "@id": "iot:Property" },
	"iot:providesOutputData": {
		"@id": "iot:VoltageData"
	},
	"iot:writable" : "schema:False",
	"iot:observable" : "schema:Boolean"
},
{
	"@id": "iot:PhaseToNeutralVoltageC",
	"@type": "rdfs:Class",
	"rdfs:comment": "The voltage between the phase (line) C and neutral (there exist phases A, B, and C).",
	"rdfs:label": "PhaseToNeutralVoltageC",
	"rdfs:subClassOf": { "@id": "iot:Property" },
	"iot:providesOutputData": {
		"@id": "iot:VoltageData"
	},
	"iot:writable" : "schema:False",
	"iot:observable" : "schema:Boolean"
},
{
	"@id": "iot:PhaseToPhaseVoltageAB",
	"@type": "rdfs:Class",
	"rdfs:comment": "The voltage between phases A and B (line-to-line voltages in a polyphase system).",
	"rdfs:label": "PhaseToPhaseVoltageAB",
	"rdfs:subClassOf": { "@id": "iot:Property" },
	"iot:providesOutputData": {
		"@id": "iot:VoltageData"
	},
	"iot:writable" : "schema:False",
	"iot:observable" : "schema:Boolean"
},
{
	"@id": "iot:PhaseToPhaseVoltageBC",
	"@type": "rdfs:Class",
	"rdfs:comment": "The voltage between phases B and C (line-to-line voltages in a polyphase system).",
	"rdfs:label": "PhaseToPhaseVoltageBC",
	"rdfs:subClassOf": { "@id": "iot:Property" },
	"iot:providesOutputData": {
		"@id": "iot:VoltageData"
	},
	"iot:writable" : "schema:False",
	"iot:observable" : "schema:Boolean"
},
{
	"@id": "iot:PhaseToPhaseVoltageCA",
	"@type": "rdfs:Class",
	"rdfs:comment": "The voltage between phases C and A (line-to-line voltages in a polyphase system).",
	"rdfs:label": "PhaseToPhaseVoltageCA",
	"rdfs:subClassOf": { "@id": "iot:Property" },
	"iot:providesOutputData": {
		"@id": "iot:VoltageData"
	},
	"iot:writable" : "schema:False",
	"iot:observable" : "schema:Boolean"
},
{
	"@id": "iot:AveragePhaseToNeutralVoltage",
	"@type": "rdfs:Class",
	"rdfs:comment": "The average voltage between phase (line) and neutral.",
	"rdfs:label": "AveragePhaseToNeutralVoltage",
	"rdfs:subClassOf": { "@id": "iot:Property" },
	"iot:providesOutputData": {
		"@id": "iot:VoltageData"
	},
	"iot:writable" : "schema:False",
	"iot:observable" : "schema:Boolean"
},
{
	"@id": "iot:AveragePhaseToPhaseVoltage",
	"@type": "rdfs:Class",
	"rdfs:comment": "The average voltage between two phases (line-to-line voltages in a polyphase system).",
	"rdfs:label": "AveragePhaseToPhaseVoltage",
	"rdfs:subClassOf": { "@id": "iot:Property" },
	"iot:providesOutputData": {
		"@id": "iot:VoltageData"
	},
	"iot:writable" : "schema:False",
	"iot:observable" : "schema:Boolean"
}
